src/program_proof/rsm/spaxos_top.v
@@ -5,3 +5,6 @@ From Perennial.program_proof Require Export grove_prelude.
 
 Definition proposals := gmap nat string.
 Definition ballot := list bool.
+Inductive consensus : Set :=
+| Chosen (v : string)
+| Free.
